<h1 style="color: #ccc">O-Level Mathematics</h1>

# Quadratic Equations

*Feb 20, 2022*

## Quadratic Equations

1. A quadratic equation is an equation with the variable of the highest power raised to two.

2. A quadratic equation is expressed in the form of

    $$
    ax^{2} +bx+c=0
    $$

3. Quadratic equations can be solved by using factorisation method, completing the square method, or quadratic formula method.

## Factorisation Method

1. Factorisation method

    **Worked Example**

    > Solve the following equation.

    $$
    2x^{2} -7x+3=0
    $$

    **Solution**

    $$
    \begin{aligned}
    2x^{2} -7x+3 & =0\\
    ( 2x-1)( x-3) & =0
    \end{aligned}\\
    $$

    $$
    \begin{aligned}
    2x-1 & =0\quad \text{or} & x-3 & =0\\
    2x & =1 & x & =3\\
    x & =\frac{1}{2} &  & 
    \end{aligned}
    $$

    Therefore, $x=\frac{1}{2}$ or $x=3$.

## Completing the Square Method

1. Completing the square method

    **Worked Example**

    > Solve the following quadratic equation using completing the square method.

    $$
    3y^{2} -5y+2 =0
    $$

    **Solution**

    $$
    \begin{aligned}
    3y^{2} -5y+2 & =0\\
    y^{2} -\frac{5}{3} y & =-\frac{2}{3}\\
    y^{2} -\frac{5}{3} y+\left( -\frac{5}{6}\right)^{2} & =-\frac{2}{3} +\left( -\frac{5}{6}\right)^{2}\\
    \left( y-\frac{5}{6}\right)^{2} & =-\frac{24}{36} +\frac{25}{36}\\
    y-\frac{5}{6} & =\pm \sqrt{\frac{1}{36}}\\
    y-\frac{5}{6} & =\pm \frac{1}{6}
    \end{aligned}\\
    $$

    $$
    \begin{aligned}
    y & =\frac{1}{6} +\frac{5}{6} \quad \text{or} & y & =-\frac{1}{6} +\frac{5}{6}\\
    y & =1 & y & =\frac{3}{2}
    \end{aligned}
    $$

    Therefore, $y=1$ or $y=\frac{3}{2}$.

## Quadratic Formula Method

1. Quadratic formula method

    **Theorem 1. (Quadratic Formula)** Given a general quadratic equation of the form

    $$
    ax^{2}+bx+c=0
    $$

    The quadratic formula to find the unknown $x$ is

    $$
    x=\frac{-b\pm \sqrt{b^{2} -4ac}}{2a}\\
    $$

    **Proof.**

    Given a general quadratic equation,

    $$
    \begin{aligned}
    ax^{2} +bx+c & =0\\
    x^{2} +\frac{b}{a} x & =-\frac{c}{a}\\
    x^{2} +\frac{b}{a} x+\left(\frac{b}{2a}\right)^{2} & =-\frac{c}{a} +\left(\frac{b}{2a}\right)^{2}\\
    \left( x+\frac{b}{2a}\right)^{2} & =\frac{b^{2} -4ac}{4a^{2}}\\
    x+\frac{b}{2a} & =\pm \frac{\sqrt{b^{2} -4ac}}{2a}\\
    x & =\pm \frac{\sqrt{b^{2} -4ac}}{2a} -\frac{b}{2a}\\
     & =\frac{-b\pm \sqrt{b^{2} -4ac}}{2a}
    \end{aligned}\\
    $$

    <p style='text-align: right;'>â– </p>

    **Worked Example**

    > Solve the following equation using quadratic formula and give your answer in 2 decimal places.

    $$
    3z^{2}=7z-1
    $$

    **Solution**

    $$
    3z^{2}-7z+1=0
    $$

    $$
    \begin{aligned}
    a & =3 & b & =-7 & c & =1
    \end{aligned}
    $$

    Using quadratic formula,

    $$
    \begin{aligned}
    z & =\frac{-b\pm \sqrt{b^{2} -4ac}}{2a}\\
     & =\frac{-( -7) \pm \sqrt{( -7)^{2} -4( 3)( 1)}}{2( 3)}\\
     & =\frac{7\pm \sqrt{37}}{6}
    \end{aligned}
    $$

    $$
    \begin{aligned}
    z & =\frac{7+\sqrt{37}}{6} \quad \text{or} & z & =\frac{7-\sqrt{37}}{6}\\
     & \approx 2.18 & & \approx -0.15
    \end{aligned}
    $$

    Therefore, $z=2.18$ or $z=-0.15$ rounding to 2 decimal places.
